some results on tree BFS

Tree.v
@@ -3,6 +3,43 @@ Import ListNotations.
 
 Require Import Regex.
 
+(** * Chaining optional results  *)
+Definition seqop {X:Type} (o1 o2: option X) : option X :=
+  match o1 with Some o => o1 | None => o2 end.
+
+Lemma seqop_none:
+  forall X (o1:option X), seqop o1 None = o1.
+Proof. intros X o1. destruct o1 eqn:O; auto. Qed.
+
+Definition seqop_list {X Y:Type} (l:list X) (f: X -> option Y) : option Y :=
+  List.fold_left (fun (y:option Y) (x:X) => seqop y (f x)) l None.
+
+Lemma app_cons:
+  forall X (h:X) l, h::l = [h] ++ l.
+Proof. intros. simpl. auto. Qed.
+
+Lemma seqop_some:
+  forall X Y l f r, List.fold_left (fun (y:option Y) (x:X) => seqop y (f x)) l (Some r) = Some r.
+Proof. intros X Y l. induction l; intros; simpl; auto. Qed.
+
+
+Lemma seqop_list_head_some:
+  forall X Y (h:X) l f (r:Y),
+    f h = Some r -> 
+    seqop_list (h::l) f = Some r.
+Proof.
+  intros X Y h l f r H. unfold seqop_list.
+  rewrite app_cons. rewrite fold_left_app.
+  simpl. rewrite H. rewrite seqop_some. auto.
+Qed.
+
+Lemma seqop_list_head_none:
+  forall X Y (h:X) l (f:X -> option Y),
+    f h = None -> 
+    seqop_list (h::l) f = seqop_list l f.
+Proof. intros. unfold seqop_list. simpl. rewrite H. auto. Qed.
+
+
 (** * Priority Trees  *)
 
 Inductive tree : Type :=
@@ -36,10 +73,7 @@ Fixpoint tree_res (t:tree) (gm:group_map): option leaf :=
   | Mismatch => None
   | Match s => Some (s, gm)
   | Choice t1 t2 =>
-      match tree_res t1 gm with
-      | None => tree_res t2 gm
-      | Some r => Some r
-      end
+      seqop (tree_res t1 gm) (tree_res t2 gm)
   | Read c t1 => tree_res t1 (add_char gm c)
   | CheckFail _ => None
   | CheckPass _ t1 => tree_res t1 gm
@@ -89,7 +123,8 @@ Theorem first_tree_leaf:
     tree_res t gm = hd_error (tree_leaves t gm).
 Proof.
   intros t. induction t; intros; simpl; auto.
-  - rewrite IHt1. rewrite IHt2. rewrite hd_error_app. auto.
+  - rewrite IHt1. rewrite IHt2. rewrite hd_error_app. unfold seqop.
+    destruct (hd_error (tree_leaves t1 gm)) eqn:HD; auto. 
 Qed.
       
 (** * Group Map irrelevance  *)
@@ -110,4 +145,127 @@ Proof.
   - apply app_eq_nil in H as [NIL1 NIL2].
     apply IHt1 with (gm2:=gm2) in NIL1. apply IHt2 with (gm2:=gm2) in NIL2.
     rewrite NIL1. rewrite NIL2. auto.
+Qed.
+
+
+
+
+
+(** * Tree BFS  *)
+(* Close to the kind of execution the PikeVM is doing on the bytecode *)
+
+(* returns three things:
+ - the list of active trees to explore next. can be empty. Each has its own group map
+ - option leaf: a result found
+ - option tree: if the tree is blocked consuming a character *)
+
+Inductive step_result : Type :=
+| StepActive: list (tree * group_map) -> step_result (* generated new active threads, possibly 0 *)
+| StepMatch: leaf -> step_result                (* a match was found *)
+| StepBlocked: tree -> step_result     (* the thread was blocked *)
+.
+
+Definition StepDead := StepActive []. (* the thread died *)
+
+Definition tree_bfs_step (t:tree) (gm:group_map): step_result :=
+  match t with
+  | Mismatch => StepDead
+  | Match i => StepMatch (i, gm)
+  | Choice t1 t2 => StepActive [(t1,gm); (t2,gm)]
+  | Read c t1 => StepBlocked t1
+  | CheckFail _ => StepDead
+  | CheckPass _ t1 => StepActive [(t1,gm)]
+  | OpenGroup gid t1 => StepActive [(t1,open_group gm gid)]
+  | CloseGroup gid t1 => StepActive [(t1, close_group gm gid)]
+  | ResetGroups gid t1 => StepActive [(t1, reset_groups gm gid)]
+  end.
+
+Definition pike_tree_state : Type :=
+  (* active, bestmatch, blocked *)
+  list (tree * group_map) * option leaf * list (tree * group_map).
+
+Definition upd_blocked {X:Type} (newblocked: option X) (blocked: list X) :=
+  match newblocked with Some b => b::blocked | None => blocked end.
+
+Inductive pike_tree_step : pike_tree_state -> pike_tree_state -> Prop :=
+| pts_nextchar:
+  (* when the list of active trees is empty, restart from the blocked ones, proceeding to the next character *)
+  forall best blocked,
+    pike_tree_step ([], best, blocked) (blocked, best, [])
+| pts_active:
+  (* generated new active trees: add them in front of the low-priority ones *)
+  forall t gm active best blocked nextactive
+    (STEP: tree_bfs_step t gm = StepActive nextactive),
+    pike_tree_step ((t,gm)::active, best, blocked) (nextactive++active, best, blocked)
+| pts_match:
+  (* a match is found, discard remaining low-priority active trees *)
+  forall t gm active best blocked leaf
+    (STEP: tree_bfs_step t gm = StepMatch leaf),
+    pike_tree_step ((t,gm)::active, best, blocked) ([], Some leaf, blocked)
+| pts_blocked:
+(* add the new blocked thread after the previous ones *)
+  forall t gm active best blocked newt
+    (STEP: tree_bfs_step t gm = StepBlocked newt),
+    pike_tree_step ((t,gm)::active, best, blocked) (active, best, blocked ++ [(newt,gm)]).
+
+Definition pike_tree_initial_state (t:tree) : pike_tree_state :=
+  ([(t, empty_group_map)], None, []).
+
+(** * Tree BFS Correction *)
+
+Definition list_result (l:list (tree * group_map)) : option leaf :=
+  seqop_list l (fun tgm => tree_res (fst tgm) (snd tgm)).
+      
+Lemma list_result_cons:
+  forall t gm l,
+    list_result ((t,gm)::l) = seqop (tree_res t gm) (list_result l).
+Proof.
+  intros. unfold list_result, seqop_list. simpl.
+Admitted.
+
+Lemma list_result_app:
+  forall l1 l2,
+    list_result (l1 ++ l2) = seqop (list_result l1) (list_result l2).
+Proof.
+Admitted.
+
+(* first, see if there is a result in blocked, then active, then take the best *)
+Definition state_result (pts: pike_tree_state) : option leaf :=
+  match pts with
+  | (active, best, blocked) =>
+      seqop (list_result blocked) (seqop (list_result active) best)
+  end.
+  
+
+(* the state result is an invariant of the pike step *)
+Theorem pts_result_preservation:
+  forall pts1 pts2,
+    pike_tree_step pts1 pts2 ->
+    state_result pts1 = state_result pts2.
+Proof.
+  intros pts1 pts2 H.
+  inversion H; subst.
+  - simpl. auto.
+  - destruct t; simpl in STEP; inversion STEP; subst.
+    + rewrite app_nil_l. unfold state_result. apply f_equal. unfold list_result. rewrite seqop_list_head_none; auto.
+    + unfold state_result. apply f_equal. apply f_equal2; auto.
+    + rewrite app_nil_l. unfold state_result. apply f_equal. unfold list_result. rewrite seqop_list_head_none; auto.
+    + unfold state_result. apply f_equal. rewrite list_result_cons. simpl. rewrite list_result_cons. auto.
+    + unfold state_result. apply f_equal. rewrite list_result_cons. simpl. rewrite list_result_cons. auto.
+    + unfold state_result. apply f_equal. rewrite list_result_cons. simpl. rewrite list_result_cons. auto.      
+    + unfold state_result. apply f_equal. rewrite list_result_cons. simpl. rewrite list_result_cons. auto.
+  - destruct t; simpl in STEP; inversion STEP; subst.
+    simpl. apply f_equal. rewrite list_result_cons. auto.
+  - destruct t; simpl in STEP; inversion STEP; subst.
+    simpl. rewrite list_result_app. rewrite list_result_cons. simpl.
+    admit.                      (* an issue with group map that must (or not? if we change group maps) change *)
+Admitted.
+
+(* the invariant is properly initialized: at the beginning, the result of the state is the first result of the tree *)
+Lemma pts_result_init:
+  forall t,
+    state_result (pike_tree_initial_state t) = first_branch t.
+Proof.
+  intros t. unfold pike_tree_initial_state, first_branch. simpl.
+  unfold list_result, seqop_list. simpl. rewrite seqop_none. auto.
 Qed.
